lexer.v
@@ -1,0 +1,101 @@
+Require Import Ascii.
+Require Import List.
+Import ListNotations.
+Require Import PeanoNat.
+Require Import Coq.Program.Wf.
+
+From VLG Require Import regex.
+
+Definition Sigma := regex.Sigma.
+Definition Sigma_dec := regex.Sigma_dec.
+Definition String := regex.String.
+
+Definition Rule : Type := String * regex.
+Definition Token : Type := String * String.
+Definition eToken : Type := Rule * String * String.
+Definition eLexemes : Type := list eToken.
+
+Fixpoint max_pref_fn (s : String) (r : regex) : option String :=
+  match s with
+  (* in a DFA approach, nullable r would instead check if the DFA is in an accept state *)
+  | [] => if nullable r then Some [] else None
+  | a :: s' =>
+    let
+      (* in a DFA approach, (derivative a r) would instead be a state transition *)
+      r' := derivative a r in
+    let
+      mpxs := max_pref_fn s' r' in
+    
+    match mpxs with
+    | None => if (nullable r') then Some [a] else None
+    | Some s'' => Some (a :: s'')
+    end
+  end.
+
+(* Maybe it would be better to build the suffix while also building the prefix? *)
+Fixpoint get_suffix (p : String) (s : String) :=
+  match p, s with
+  | [], _ => Some s (* p consumed, the rest is suffix *)
+  | _, [] => None (* p longer than s *)
+  | b::bs, c::cs => if Sigma_dec b c then get_suffix bs cs
+                 else None (* if characters don't match up point-wise, p is not a prefix *)
+  end.
+
+(* couldn't find this in the list library? *)
+Fixpoint fold {X Y: Type} (f: X->Y->Y) (l: list X) (b: Y)
+                         : Y :=
+  match l with
+  | nil => b
+  | h :: t => f h (fold f t b)
+  end.
+
+(* 
+   This function will accept a list of pairs and a string.
+   Each element in this list of pairs will contain a regex and its corresponding label/action.
+
+   The function will return a list of triples.
+   Each element in this list of triples will be of the form ((a, re), pre, suff).
+   The tokens can be extracted as (a, pref), where a is the label/action and 
+     pre is the labeled word.
+
+   The additional elements in the triple might be helpful for correctness.
+
+   0. An error will be thrown <-> the code could not be lexed entirely according to the rules
+   In all cases where an error is not thrown:
+   1. exp_match pref re
+   2. the concatention of all pre is equal to code
+   3. If suff = x ++ y, then pre ++ x does not match any of the regular expressions from rules
+ *)
+Program Fixpoint lex (rules : list Rule) (code : String) {measure (length code)} : list eToken :=
+  match code with
+  | [] => []
+  | _ =>
+    let (* find all the maximal prefixes, associating them with a rule as we go *)
+      mprefs := map (fun ru => match ru with (a, re) => ((a, re), max_pref_fn code re) end) rules
+    in
+    let (* of these maximal prefixes, find the longest *)
+      mpref := fold (fun apref1 apref2 =>
+                       match apref1, apref2 with
+                       | (_, None), (_, _) => apref2
+                       | (_, _), (_, None) => apref1
+                       | (_, Some x), (_, Some y) => if (length y) <? (length x)
+                                                    then apref2 else apref1
+                       end
+                    ) mprefs (([], EmptySet), None)
+    in
+    let (* get the associated suffix -- might be better to build this while building the prefix? *)
+      msuff := match mpref with
+                    | (_, None) => None (* This state suggests malformed code *)
+                    | (_, Some x) => get_suffix x code
+               end
+    in
+    match mpref, msuff with
+    | (_, None), _ => [] (* This state suggests malformed code *)
+    | _, None => [] (* This state suggests malformed code *)
+    | (ru, Some prefix), Some suffix => (ru, prefix, suffix) :: (lex rules suffix)
+    end
+      
+  end.
+                 
+  
+  
